proved client of increment with ghost state

ghost_state_simple.v
@@ -101,13 +101,13 @@ Section GhostStateSimple.
     admit.
   Admitted.
 
-  Definition inc_invariant N γ (l : loc) (n : Z) : iProp Σ := inv N (∃(k:Z), l ↦ #k ∗ ((own γ S ∧ ⌜k >= n⌝) ∨ (own γ F ∧ ⌜k >= n + 1⌝)))%I.
+  Definition inc_invariant γ (l : loc) (n : Z) : iProp Σ := (∃(k:Z), l ↦ #k ∗ ((own γ S ∧ ⌜k >= n⌝) ∨ (own γ F ∧ ⌜k >= n + 1⌝)))%I.
 
   Definition prog_inc (l : loc) : expr :=
     #l <- !#l + #1.
 
   Lemma prog_inc_wp N γ l n:
-    inc_invariant N γ l n -∗ {{{ ⌜True ⌝}}} prog_inc l {{{ v, RET v; own γ F }}}.
+    inv N (inc_invariant γ l n) -∗ {{{ ⌜True ⌝}}} prog_inc l {{{ v, RET v; own γ F }}}.
   Proof.
     iIntros "#Hinv".
     iIntros (Φ). iModIntro.
@@ -120,7 +120,9 @@ Section GhostStateSimple.
     iDestruct "Hl" as (k) "(Hl & Hghost)".
     iAssert (⌜k >= n⌝)%I as "%".
     { iDestruct "Hghost" as "[[Htok Hbound]|[Htok Hbound]]";
-        iDestruct "Hbound" as %Hbound; (* Coq hung here if I used "%" *)
+        iDestruct "Hbound" as %Hbound; (* Coq hung here if I used "%",
+        probably because there is another branch using the same name
+        Hbound *)
         iPureIntro;
         omega. }
     wp_load.
@@ -152,7 +154,6 @@ Section GhostStateSimple.
       (* close the invariant using Htok2 *)
       iMod ("cl" with "[Hl Htok2]") as "_".
       { iModIntro. iExists (k + 1). iFrame. auto. }
-      iModIntro.
       iApply ("HΦ" with "[$Htok1]").
     - (* own F: no need to do a frame preserving update since we can
       just duplicate our token. *)
@@ -160,6 +161,43 @@ Section GhostStateSimple.
       iMod ("cl" with "[Hl Htok2]") as "_".
       { iModIntro. iExists (k + 1). iFrame. auto. }
       iApply ("HΦ" with "[$Htok1]").
+  Qed.
+
+  Lemma prog_client_wp (l : loc) (n : Z):
+    {{{ l ↦ #n }}} prog_inc l;; !#l {{{ v, RET v; ⌜∃k:Z, v = #k ∧ k >= n + 1⌝ }}}.
+  Proof using incG0. (* not sure what this is for, but Coq was complaining about it *)
+    iIntros (Φ) "Hl HΦ".
+    (* allocate ghost state token, for which we have to show ✓ S. *)
+    iMod (own_alloc S) as (γ) "Htok"; first split.
+    (* allocate the invariant *)
+    iMod (inv_alloc (nroot.@"client") _ (inc_invariant γ l n) with "[Hl Htok]") as "#Hinv".
+    { (* initially establish invariant *)
+      assert (n >= n) by omega. iModIntro. rewrite /inc_invariant.
+      iExists n. iFrame. auto. }
+    wp_bind (prog_inc l)%E.
+    iApply prog_inc_wp; try done.
+    iModIntro.
+    iIntros (v) "Htok".
+    wp_seq.
+    (* wasn't able to open the invariant again to show the conclusion
+    if I didn't put the skip instruction after prog_inc. Makes sense
+    because we need an atomic instruction. *)
+    iInv "Hinv" as "Hl" "cl".
+    iMod "Hl".
+    rewrite /inc_invariant.
+    iDestruct "Hl" as (k) "[Hl [[Htok1 Hbound]|[Htok2 Hbound]]]".
+    - (* own S and own F are incompatible, hence we cannot be in this case *)
+      iExFalso.
+      iApply (incRA_S_F_incompatible with "[$Htok1 $Htok]").
+    - (* Here we have the desired bound due to the case of the invariant we are in *)
+      iDestruct "Hbound" as "%".
+      wp_load.
+      iMod ("cl" with "[Htok2 Hl]") as "_".
+      { iModIntro. iExists k. iFrame. auto. }
+      iModIntro.
+      iApply "HΦ".
+      iPureIntro.
+      by exists k.
   Qed.
 
 End GhostStateSimple.
